ems/SimModSem.v
@@ -31,124 +31,124 @@ Local Open Scope nat_scope.
 
 
 Section SIM.
-  (* Let st_local: Type := (Any.t). *)
+  Let st_local: Type := (Any.t).
 
   Variable world: Type.
 
-  (* Let W: Type := (Any.t) * (Any.t). *)
-  (* Variable wf : world -> W -> Prop. *)
+  Let W: Type := (Any.t) * (Any.t).
+  Variable wf : world -> W -> Prop.
   Variable le: relation world.
 
 
-  Inductive _sim_itree (sim_itree: forall (st_src st_tgt R_src R_tgt: Type) (wf: world -> (st_src * st_tgt) -> Prop) (RR: st_src -> st_tgt -> R_src -> R_tgt -> Prop), bool -> bool -> world -> st_src * itree (Es st_src) R_src -> st_tgt * itree (Es st_tgt) R_tgt -> Prop)
-          {st_src st_tgt R_src R_tgt} (wf: world -> (st_src * st_tgt) -> Prop) (RR: st_src -> st_tgt -> R_src -> R_tgt -> Prop)
-    : bool -> bool -> world -> st_src * itree (Es st_src) R_src -> st_tgt * itree (Es st_tgt) R_tgt -> Prop :=
+  Inductive _sim_itree (sim_itree: forall (R_src R_tgt: Type) (RR: st_local -> st_local -> R_src -> R_tgt -> Prop), bool -> bool -> world -> st_local * itree Es R_src -> st_local * itree Es R_tgt -> Prop)
+          {R_src R_tgt} (RR: st_local -> st_local -> R_src -> R_tgt -> Prop)
+    : bool -> bool -> world -> st_local * itree Es R_src -> st_local * itree Es R_tgt -> Prop :=
   | sim_itree_ret
       i_src0 i_tgt0 w0 st_src0 st_tgt0
       v_src v_tgt
       (RET: RR st_src0 st_tgt0 v_src v_tgt)
     :
-      _sim_itree sim_itree wf RR i_src0 i_tgt0 w0 (st_src0, Ret v_src) (st_tgt0, Ret v_tgt)
+      _sim_itree sim_itree RR i_src0 i_tgt0 w0 (st_src0, Ret v_src) (st_tgt0, Ret v_tgt)
 
   | sim_itree_call
       i_src0 i_tgt0 w w0 st_src0 st_tgt0
       fn varg k_src k_tgt
       (WF: wf w0 (st_src0, st_tgt0))
       (K: forall w1 vret st_src1 st_tgt1 (WLE: le w0 w1) (WF: wf w1 (st_src1, st_tgt1)),
-          sim_itree _ _ _ _ wf RR false false w (st_src1, k_src vret) (st_tgt1, k_tgt vret))
+          sim_itree _ _ RR false false w (st_src1, k_src vret) (st_tgt1, k_tgt vret))
     :
-      _sim_itree sim_itree wf RR i_src0 i_tgt0 w (st_src0, trigger (Call fn varg) >>= k_src)
+      _sim_itree sim_itree RR i_src0 i_tgt0 w (st_src0, trigger (Call fn varg) >>= k_src)
                  (st_tgt0, trigger (Call fn varg) >>= k_tgt)
 
   | sim_itree_syscall
       i_src0 i_tgt0 w0 st_src0 st_tgt0
       fn varg rvs k_src k_tgt
       (K: forall vret,
-          sim_itree _ _ _ _ wf RR true true w0 (st_src0, k_src vret) (st_tgt0, k_tgt vret))
+          sim_itree _ _ RR true true w0 (st_src0, k_src vret) (st_tgt0, k_tgt vret))
     :
-      _sim_itree sim_itree wf RR i_src0 i_tgt0 w0 (st_src0, trigger (Syscall fn varg rvs) >>= k_src)
+      _sim_itree sim_itree RR i_src0 i_tgt0 w0 (st_src0, trigger (Syscall fn varg rvs) >>= k_src)
                  (st_tgt0, trigger (Syscall fn varg rvs) >>= k_tgt)
 
   | sim_itree_tau_src
-      i_src0 i_tgt0 w0 (st_src0: st_src) (st_tgt0: st_tgt)
+      i_src0 i_tgt0 w0 (st_src0: st_local) (st_tgt0: st_local)
       i_src i_tgt
-      (K: _sim_itree sim_itree wf RR true i_tgt0 w0 (st_src0, i_src) (st_tgt0, i_tgt))
+      (K: _sim_itree sim_itree RR true i_tgt0 w0 (st_src0, i_src) (st_tgt0, i_tgt))
     :
-      _sim_itree sim_itree wf RR i_src0 i_tgt0 w0 (st_src0, tau;; i_src) (st_tgt0, i_tgt)
+      _sim_itree sim_itree RR i_src0 i_tgt0 w0 (st_src0, tau;; i_src) (st_tgt0, i_tgt)
 
   | sim_itree_tau_tgt
-      i_src0 i_tgt0 w0 (st_src0: st_src) (st_tgt0: st_tgt)
+      i_src0 i_tgt0 w0 (st_src0: st_local) (st_tgt0: st_local)
       i_src i_tgt
-      (K: _sim_itree sim_itree wf RR i_src0 true w0 (st_src0, i_src) (st_tgt0, i_tgt))
+      (K: _sim_itree sim_itree RR i_src0 true w0 (st_src0, i_src) (st_tgt0, i_tgt))
     :
-      _sim_itree sim_itree wf RR i_src0 i_tgt0 w0 (st_src0, i_src) (st_tgt0, tau;; i_tgt)
+      _sim_itree sim_itree RR i_src0 i_tgt0 w0 (st_src0, i_src) (st_tgt0, tau;; i_tgt)
 
   | sim_itree_choose_src
-      i_src0 i_tgt0 w0 (st_src0: st_src) (st_tgt0: st_tgt)
+      i_src0 i_tgt0 w0 (st_src0: st_local) (st_tgt0: st_local)
       X k_src i_tgt
-      (K: exists (x: X), _sim_itree sim_itree wf RR true i_tgt0 w0 (st_src0, k_src x) (st_tgt0, i_tgt))
+      (K: exists (x: X), _sim_itree sim_itree RR true i_tgt0 w0 (st_src0, k_src x) (st_tgt0, i_tgt))
     :
-      _sim_itree sim_itree wf RR i_src0 i_tgt0 w0 (st_src0, trigger (Choose X) >>= k_src)
+      _sim_itree sim_itree RR i_src0 i_tgt0 w0 (st_src0, trigger (Choose X) >>= k_src)
                  (st_tgt0, i_tgt)
 
   | sim_itree_choose_tgt
-      i_src0 i_tgt0 w0 (st_src0: st_src) (st_tgt0: st_tgt)
+      i_src0 i_tgt0 w0 (st_src0: st_local) (st_tgt0: st_local)
       X i_src k_tgt
-      (K: forall (x: X), _sim_itree sim_itree wf RR i_src0 true w0 (st_src0, i_src) (st_tgt0, k_tgt x))
+      (K: forall (x: X), _sim_itree sim_itree RR i_src0 true w0 (st_src0, i_src) (st_tgt0, k_tgt x))
     :
-      _sim_itree sim_itree wf RR i_src0 i_tgt0 w0 (st_src0, i_src)
+      _sim_itree sim_itree RR i_src0 i_tgt0 w0 (st_src0, i_src)
                  (st_tgt0, trigger (Choose X) >>= k_tgt)
 
   | sim_itree_take_src
-      i_src0 i_tgt0 w0 (st_src0: st_src) (st_tgt0: st_tgt)
+      i_src0 i_tgt0 w0 (st_src0: st_local) (st_tgt0: st_local)
       X k_src i_tgt
-      (K: forall (x: X), _sim_itree sim_itree wf RR true i_tgt0 w0 (st_src0, k_src x) (st_tgt0, i_tgt))
+      (K: forall (x: X), _sim_itree sim_itree RR true i_tgt0 w0 (st_src0, k_src x) (st_tgt0, i_tgt))
     :
-      _sim_itree sim_itree wf RR i_src0 i_tgt0 w0 (st_src0, trigger (Take X) >>= k_src)
+      _sim_itree sim_itree RR i_src0 i_tgt0 w0 (st_src0, trigger (Take X) >>= k_src)
                  (st_tgt0, i_tgt)
 
   | sim_itree_take_tgt
-      i_src0 i_tgt0 w0 (st_src0: st_src) (st_tgt0: st_tgt)
+      i_src0 i_tgt0 w0 (st_src0: st_local) (st_tgt0: st_local)
       X i_src k_tgt
-      (K: exists (x: X), _sim_itree sim_itree wf RR i_src0 true w0 (st_src0, i_src) (st_tgt0, k_tgt x))
+      (K: exists (x: X), _sim_itree sim_itree RR i_src0 true w0 (st_src0, i_src) (st_tgt0, k_tgt x))
     :
-      _sim_itree sim_itree wf RR i_src0 i_tgt0 w0 (st_src0, i_src)
+      _sim_itree sim_itree RR i_src0 i_tgt0 w0 (st_src0, i_src)
                  (st_tgt0, trigger (Take X) >>= k_tgt)
 
   | sim_itree_supdate_src
-      i_src0 i_tgt0 w0 (st_src0: st_src) (st_tgt0: st_tgt)
+      i_src0 i_tgt0 w0 (st_src0: st_local) (st_tgt0: st_local)
       X k_src i_tgt
-      (run: st_src -> st_src * X )
-      (K: _sim_itree sim_itree wf RR true i_tgt0 w0 (fst (run st_src0), k_src (snd (run st_src0))) (st_tgt0, i_tgt))
+      (run: st_local -> st_local * X )
+      (K: _sim_itree sim_itree RR true i_tgt0 w0 (fst (run st_src0), k_src (snd (run st_src0))) (st_tgt0, i_tgt))
     :
-      _sim_itree sim_itree wf RR i_src0 i_tgt0 w0 (st_src0, trigger (SUpdate run) >>= k_src) (st_tgt0, i_tgt)  
+      _sim_itree sim_itree RR i_src0 i_tgt0 w0 (st_src0, trigger (SUpdate run) >>= k_src) (st_tgt0, i_tgt)  
 
   | sim_itree_supdate_tgt
-      i_src0 i_tgt0 w0 (st_src0: st_src) (st_tgt0: st_tgt)
+      i_src0 i_tgt0 w0 (st_src0: st_local) (st_tgt0: st_local)
       X i_src k_tgt
-      (run: st_tgt -> st_tgt * X )
-      (K: _sim_itree sim_itree wf RR i_src0 true w0 (st_src0, i_src) (fst (run st_tgt0), k_tgt (snd (run st_tgt0))))
+      (run: st_local -> st_local * X )
+      (K: _sim_itree sim_itree RR i_src0 true w0 (st_src0, i_src) (fst (run st_tgt0), k_tgt (snd (run st_tgt0))))
     :
-      _sim_itree sim_itree wf RR i_src0 i_tgt0 w0 (st_src0, i_src) (st_tgt0, trigger (SUpdate run) >>= k_tgt)
+      _sim_itree sim_itree RR i_src0 i_tgt0 w0 (st_src0, i_src) (st_tgt0, trigger (SUpdate run) >>= k_tgt)
 
   | sim_itree_progress
-      i_src0 i_tgt0 w0 (st_src0: st_src) (st_tgt0: st_tgt) i_src i_tgt
-      (SIM: sim_itree _ _ _ _ wf RR false false w0 (st_src0, i_src) (st_tgt0, i_tgt))
+      i_src0 i_tgt0 w0 (st_src0: st_local) (st_tgt0: st_local) i_src i_tgt
+      (SIM: sim_itree _ _ RR false false w0 (st_src0, i_src) (st_tgt0, i_tgt))
       (SRC: i_src0 = true)
       (TGT: i_tgt0 = true)
     :
-      _sim_itree sim_itree wf RR true true w0 (st_src0, i_src) (st_tgt0, i_tgt)
+      _sim_itree sim_itree RR true true w0 (st_src0, i_src) (st_tgt0, i_tgt)
   .
 
-  Definition lift_rel {st_src st_tgt R_src R_tgt} (w0: world) (wf: world -> (st_src * st_tgt) -> Prop) (RR: R_src -> R_tgt -> Prop)
-             (st_src0: st_src) (st_tgt0: st_tgt) (ret_src ret_tgt: Any.t) :=
+  Definition lift_rel {R_src R_tgt} (w0: world) (RR: R_src -> R_tgt -> Prop)
+             (st_src0: st_local) (st_tgt0: st_local) (ret_src ret_tgt: Any.t) :=
     exists w1 : world,
       (<<WLE: le w0 w1 >> /\ <<WF: wf w1 (st_src0, st_tgt0) >> /\ <<RET: ret_src = ret_tgt >>).
 
-  Lemma _sim_itree_ind2 (sim_itree: forall (st_src st_tgt R_src R_tgt: Type) (wf: world -> (st_src * st_tgt) -> Prop) 
-                                    (RR: st_src -> st_tgt -> R_src -> R_tgt -> Prop), bool -> bool -> world -> st_src * itree (Es st_src) R_src -> st_tgt * itree (Es st_tgt) R_tgt -> Prop)
-        {st_src st_tgt R_src R_tgt} (wf: world -> (st_src * st_tgt) -> Prop) (RR: st_src -> st_tgt -> R_src -> R_tgt -> Prop)
-        (P: bool -> bool -> world -> st_src * itree (Es st_src) R_src -> st_tgt * itree (Es st_tgt) R_tgt -> Prop)
+  Lemma _sim_itree_ind2 (sim_itree: forall (R_src R_tgt: Type) 
+                                    (RR: st_local -> st_local -> R_src -> R_tgt -> Prop), bool -> bool -> world -> st_local * itree Es R_src -> st_local * itree Es R_tgt -> Prop)
+        {R_src R_tgt} (RR: st_local -> st_local -> R_src -> R_tgt -> Prop)
+        (P: bool -> bool -> world -> st_local * itree Es R_src -> st_local * itree Es R_tgt -> Prop)
         (RET: forall
             i_src0 i_tgt0 w0 st_src0 st_tgt0
             v_src v_tgt
@@ -159,75 +159,75 @@ Section SIM.
             fn varg k_src k_tgt
             (WF: wf w0 (st_src0, st_tgt0))
             (K: forall w1 vret st_src1 st_tgt1 (WLE: le w0 w1) (WF: wf w1 (st_src1, st_tgt1)),
-                sim_itree _ _ _ _ wf RR false false w (st_src1, k_src vret) (st_tgt1, k_tgt vret)),
+                sim_itree _ _ RR false false w (st_src1, k_src vret) (st_tgt1, k_tgt vret)),
             P i_src0 i_tgt0 w (st_src0, trigger (Call fn varg) >>= k_src)
               (st_tgt0, trigger (Call fn varg) >>= k_tgt))
         (SYSCALL: forall
-            i_src0 i_tgt0 w0 (st_src0: st_src) (st_tgt0: st_tgt)
+            i_src0 i_tgt0 w0 (st_src0: st_local) (st_tgt0: st_local)
             fn varg rvs k_src k_tgt
             (K: forall vret,
-                sim_itree _ _ _ _ wf RR true true w0 (st_src0, k_src vret) (st_tgt0, k_tgt vret)),
+                sim_itree _ _ RR true true w0 (st_src0, k_src vret) (st_tgt0, k_tgt vret)),
             P i_src0 i_tgt0 w0 (st_src0, trigger (Syscall fn varg rvs) >>= k_src)
               (st_tgt0, trigger (Syscall fn varg rvs) >>= k_tgt))
         (TAUSRC: forall
-            i_src0 i_tgt0 w0 (st_src0: st_src) (st_tgt0: st_tgt)
+            i_src0 i_tgt0 w0 (st_src0: st_local) (st_tgt0: st_local)
             i_src i_tgt
-            (K: _sim_itree sim_itree wf RR true i_tgt0 w0 (st_src0, i_src) (st_tgt0, i_tgt))
+            (K: _sim_itree sim_itree RR true i_tgt0 w0 (st_src0, i_src) (st_tgt0, i_tgt))
             (IH: P true i_tgt0 w0 (st_src0, i_src) (st_tgt0, i_tgt)),
             P i_src0 i_tgt0 w0 (st_src0, tau;; i_src) (st_tgt0, i_tgt))
         (TAUTGT: forall
-            i_src0 i_tgt0 w0 (st_src0: st_src) (st_tgt0: st_tgt)
+            i_src0 i_tgt0 w0 (st_src0: st_local) (st_tgt0: st_local)
             i_src i_tgt
-            (K: _sim_itree sim_itree wf RR i_src0 true w0 (st_src0, i_src) (st_tgt0, i_tgt))
+            (K: _sim_itree sim_itree RR i_src0 true w0 (st_src0, i_src) (st_tgt0, i_tgt))
             (IH: P i_src0 true w0 (st_src0, i_src) (st_tgt0, i_tgt)),
             P i_src0 i_tgt0 w0 (st_src0, i_src) (st_tgt0, tau;; i_tgt))
         (CHOOSESRC: forall
-            i_src0 i_tgt0 w0 (st_src0: st_src) (st_tgt0: st_tgt)
+            i_src0 i_tgt0 w0 (st_src0: st_local) (st_tgt0: st_local)
             X k_src i_tgt
-            (K: exists (x: X), <<SIM: _sim_itree sim_itree wf RR true i_tgt0 w0 (st_src0, k_src x) (st_tgt0, i_tgt)>> /\ <<IH: P true i_tgt0 w0 (st_src0, k_src x) (st_tgt0, i_tgt)>>),
+            (K: exists (x: X), <<SIM: _sim_itree sim_itree RR true i_tgt0 w0 (st_src0, k_src x) (st_tgt0, i_tgt)>> /\ <<IH: P true i_tgt0 w0 (st_src0, k_src x) (st_tgt0, i_tgt)>>),
             P i_src0 i_tgt0 w0 (st_src0, trigger (Choose X) >>= k_src)
               (st_tgt0, i_tgt))
         (CHOOSETGT: forall
-            i_src0 i_tgt0 w0 (st_src0: st_src) (st_tgt0: st_tgt)
+            i_src0 i_tgt0 w0 (st_src0: st_local) (st_tgt0: st_local)
             X i_src k_tgt
-            (K: forall (x: X), <<SIMH: _sim_itree sim_itree wf RR i_src0 true w0 (st_src0, i_src) (st_tgt0, k_tgt x)>> /\ <<IH: P i_src0 true w0 (st_src0, i_src) (st_tgt0, k_tgt x)>>),
+            (K: forall (x: X), <<SIMH: _sim_itree sim_itree RR i_src0 true w0 (st_src0, i_src) (st_tgt0, k_tgt x)>> /\ <<IH: P i_src0 true w0 (st_src0, i_src) (st_tgt0, k_tgt x)>>),
             P i_src0 i_tgt0 w0 (st_src0, i_src)
               (st_tgt0, trigger (Choose X) >>= k_tgt))
         (TAKESRC: forall
-            i_src0 i_tgt0 w0 (st_src0: st_src) (st_tgt0: st_tgt)
+            i_src0 i_tgt0 w0 (st_src0: st_local) (st_tgt0: st_local)
             X k_src i_tgt
-            (K: forall (x: X), <<SIM: _sim_itree sim_itree wf RR true i_tgt0 w0 (st_src0, k_src x) (st_tgt0, i_tgt)>> /\ <<IH: P true i_tgt0 w0 (st_src0, k_src x) (st_tgt0, i_tgt)>>),
+            (K: forall (x: X), <<SIM: _sim_itree sim_itree RR true i_tgt0 w0 (st_src0, k_src x) (st_tgt0, i_tgt)>> /\ <<IH: P true i_tgt0 w0 (st_src0, k_src x) (st_tgt0, i_tgt)>>),
             P i_src0 i_tgt0 w0 (st_src0, trigger (Take X) >>= k_src)
               (st_tgt0, i_tgt))
         (TAKETGT: forall
-            i_src0 i_tgt0 w0 (st_src0: st_src) (st_tgt0: st_tgt)
+            i_src0 i_tgt0 w0 (st_src0: st_local) (st_tgt0: st_local)
             X i_src k_tgt
-            (K: exists (x: X), <<SIM:_sim_itree sim_itree wf RR i_src0 true w0 (st_src0, i_src) (st_tgt0, k_tgt x)>> /\ <<IH: P i_src0 true w0 (st_src0, i_src) (st_tgt0, k_tgt x)>>),
+            (K: exists (x: X), <<SIM:_sim_itree sim_itree RR i_src0 true w0 (st_src0, i_src) (st_tgt0, k_tgt x)>> /\ <<IH: P i_src0 true w0 (st_src0, i_src) (st_tgt0, k_tgt x)>>),
             P i_src0 i_tgt0 w0 (st_src0, i_src)
               (st_tgt0, trigger (Take X) >>= k_tgt))
         (SUPDATESRC: forall
-            i_src0 i_tgt0 w0 (st_src0: st_src) (st_tgt0: st_tgt)
+            i_src0 i_tgt0 w0 (st_src0: st_local) (st_tgt0: st_local)
             X k_src i_tgt
-            (run: st_src -> st_src * X )
-            (K: _sim_itree sim_itree wf RR true i_tgt0 w0 (fst (run st_src0), k_src (snd (run st_src0))) (st_tgt0, i_tgt))
+            (run: st_local -> st_local * X )
+            (K: _sim_itree sim_itree RR true i_tgt0 w0 (fst (run st_src0), k_src (snd (run st_src0))) (st_tgt0, i_tgt))
             (IH: P true i_tgt0 w0 (fst (run st_src0), k_src (snd (run st_src0))) (st_tgt0, i_tgt)),
             P i_src0 i_tgt0 w0 (st_src0, trigger (SUpdate run) >>= k_src) (st_tgt0, i_tgt))
         (SUPDATETGT: forall
-            i_src0 i_tgt0 w0 (st_src0: st_src) (st_tgt0: st_tgt)
+            i_src0 i_tgt0 w0 (st_src0: st_local) (st_tgt0: st_local)
             X i_src k_tgt
-            (run: st_tgt -> st_tgt * X )
-            (K: _sim_itree sim_itree wf RR i_src0 true w0 (st_src0, i_src) (fst (run st_tgt0), k_tgt (snd (run st_tgt0))))
+            (run: st_local -> st_local * X )
+            (K: _sim_itree sim_itree RR i_src0 true w0 (st_src0, i_src) (fst (run st_tgt0), k_tgt (snd (run st_tgt0))))
             (IH: P i_src0 true w0 (st_src0, i_src) (fst (run st_tgt0), k_tgt (snd (run st_tgt0)))),
             P i_src0 i_tgt0 w0 (st_src0, i_src) (st_tgt0, trigger (SUpdate run) >>= k_tgt))
         (PROGRESS: forall
-            i_src0 i_tgt0 w0 (st_src0: st_src) (st_tgt0: st_tgt) i_src i_tgt
-            (SIM: sim_itree _ _ _ _ wf RR false false w0 (st_src0, i_src) (st_tgt0, i_tgt))
+            i_src0 i_tgt0 w0 (st_src0: st_local) (st_tgt0: st_local) i_src i_tgt
+            (SIM: sim_itree _ _ RR false false w0 (st_src0, i_src) (st_tgt0, i_tgt))
             (SRC: i_src0 = true)
             (TGT: i_tgt0 = true),
             P true true w0 (st_src0, i_src) (st_tgt0, i_tgt))
     :
       forall i_src0 i_tgt0 w0 st_src st_tgt
-             (SIM: _sim_itree sim_itree wf RR i_src0 i_tgt0 w0 st_src st_tgt),
+             (SIM: _sim_itree sim_itree RR i_src0 i_tgt0 w0 st_src st_tgt),
         P i_src0 i_tgt0 w0 st_src st_tgt.
   Proof.
     fix IH 6. i. inv SIM.
@@ -246,10 +246,10 @@ Section SIM.
 
   Qed.
 
-  Definition sim_itree {st_src st_tgt} o_src o_tgt w0 (wf: world -> (st_src * st_tgt) -> Prop): _ -> _ -> Prop :=
-    paco11 _sim_itree bot11 _ _ _ _ wf (lift_rel w0 wf (@eq Any.t)) o_src o_tgt w0.
+  Definition sim_itree o_src o_tgt w0 : relation _ :=
+    paco8 _sim_itree bot8 _ _ (lift_rel w0 (@eq Any.t)) o_src o_tgt w0.
 
-  Lemma sim_itree_mon: monotone11 _sim_itree.
+  Lemma sim_itree_mon: monotone8 _sim_itree.
   Proof.
     ii. induction IN using _sim_itree_ind2; try (by des; econs; ss; et).
     - econs; ss; et. ii. exploit K; et. i; des. esplits; et.
@@ -259,11 +259,11 @@ Section SIM.
   Hint Constructors _sim_itree.
   Hint Unfold sim_itree.
   Hint Resolve sim_itree_mon: paco.
-  Hint Resolve cpn11_wcompat: paco.
+  Hint Resolve cpn8_wcompat: paco.
 
   Lemma sim_itree_ind
-        {st_src st_tgt} R_src R_tgt (wf: world -> (st_src * st_tgt) -> Prop) (RR: st_src -> st_tgt -> R_src -> R_tgt -> Prop) 
-        (P: bool -> bool -> world -> st_src * itree (Es st_src) R_src -> st_tgt * itree (Es st_tgt) R_tgt -> Prop)
+        R_src R_tgt (RR: st_local -> st_local -> R_src -> R_tgt -> Prop) 
+        (P: bool -> bool -> world -> st_local * itree Es R_src -> st_local * itree Es R_tgt -> Prop)
         (RET: forall
             i_src0 i_tgt0 w0 st_src0 st_tgt0
             v_src v_tgt
@@ -274,77 +274,77 @@ Section SIM.
             fn varg k_src k_tgt
             (WF: wf w0 (st_src0, st_tgt0))
             (K: forall w1 vret st_src1 st_tgt1 (WLE: le w0 w1) (WF: wf w1 (st_src1, st_tgt1)),
-                paco11 _sim_itree bot11 _ _ _ _ wf RR false false w (st_src1, k_src vret) (st_tgt1, k_tgt vret)),
+                paco8 _sim_itree bot8 _ _ RR false false w (st_src1, k_src vret) (st_tgt1, k_tgt vret)),
             P i_src0 i_tgt0 w (st_src0, trigger (Call fn varg) >>= k_src)
               (st_tgt0, trigger (Call fn varg) >>= k_tgt))
         (SYSCALL: forall
-            i_src0 i_tgt0 w0 (st_src0: st_src) (st_tgt0: st_tgt)
+            i_src0 i_tgt0 w0 (st_src0: st_local) (st_tgt0: st_local)
             fn varg rvs k_src k_tgt
             (K: forall vret,
-                paco11 _sim_itree bot11 _ _ _ _ wf RR true true w0 (st_src0, k_src vret) (st_tgt0, k_tgt vret)),
+                paco8 _sim_itree bot8 _ _ RR true true w0 (st_src0, k_src vret) (st_tgt0, k_tgt vret)),
             P i_src0 i_tgt0 w0 (st_src0, trigger (Syscall fn varg rvs) >>= k_src)
               (st_tgt0, trigger (Syscall fn varg rvs) >>= k_tgt))
         (TAUSRC: forall
-            i_src0 i_tgt0 w0 (st_src0: st_src) (st_tgt0: st_tgt)
+            i_src0 i_tgt0 w0 (st_src0: st_local) (st_tgt0: st_local)
             i_src i_tgt
-            (K: paco11 _sim_itree bot11 _ _ _ _ wf RR true i_tgt0 w0 (st_src0, i_src) (st_tgt0, i_tgt))
+            (K: paco8 _sim_itree bot8 _ _ RR true i_tgt0 w0 (st_src0, i_src) (st_tgt0, i_tgt))
             (IH: P true i_tgt0 w0 (st_src0, i_src) (st_tgt0, i_tgt)),
             P i_src0 i_tgt0 w0 (st_src0, tau;; i_src) (st_tgt0, i_tgt))
         (TAUTGT: forall
-            i_src0 i_tgt0 w0 (st_src0: st_src) (st_tgt0: st_tgt)
+            i_src0 i_tgt0 w0 (st_src0: st_local) (st_tgt0: st_local)
             i_src i_tgt
-            (K: paco11 _sim_itree bot11 _ _ _ _ wf RR i_src0 true w0 (st_src0, i_src) (st_tgt0, i_tgt))
+            (K: paco8 _sim_itree bot8 _ _ RR i_src0 true w0 (st_src0, i_src) (st_tgt0, i_tgt))
             (IH: P i_src0 true w0 (st_src0, i_src) (st_tgt0, i_tgt)),
             P i_src0 i_tgt0 w0 (st_src0, i_src) (st_tgt0, tau;; i_tgt))            
         (CHOOSESRC: forall
-            i_src0 i_tgt0 w0 (st_src0: st_src) (st_tgt0: st_tgt)
+            i_src0 i_tgt0 w0 (st_src0: st_local) (st_tgt0: st_local)
             X k_src i_tgt
-            (K: exists (x: X), <<SIM: paco11 _sim_itree bot11 _ _ _ _ wf RR true i_tgt0 w0 (st_src0, k_src x) (st_tgt0, i_tgt)>> /\ <<IH: P true i_tgt0 w0 (st_src0, k_src x) (st_tgt0, i_tgt)>>),
+            (K: exists (x: X), <<SIM: paco8 _sim_itree bot8 _ _ RR true i_tgt0 w0 (st_src0, k_src x) (st_tgt0, i_tgt)>> /\ <<IH: P true i_tgt0 w0 (st_src0, k_src x) (st_tgt0, i_tgt)>>),
             P i_src0 i_tgt0 w0 (st_src0, trigger (Choose X) >>= k_src)
               (st_tgt0, i_tgt))
         (CHOOSETGT: forall
-            i_src0 i_tgt0 w0 (st_src0: st_src) (st_tgt0: st_tgt)
+            i_src0 i_tgt0 w0 (st_src0: st_local) (st_tgt0: st_local)
             X i_src k_tgt
-            (K: forall (x: X), <<SIMH: paco11 _sim_itree bot11 _ _ _ _ wf RR i_src0 true w0 (st_src0, i_src) (st_tgt0, k_tgt x)>> /\ <<IH: P i_src0 true w0 (st_src0, i_src) (st_tgt0, k_tgt x)>>),
+            (K: forall (x: X), <<SIMH: paco8 _sim_itree bot8 _ _ RR i_src0 true w0 (st_src0, i_src) (st_tgt0, k_tgt x)>> /\ <<IH: P i_src0 true w0 (st_src0, i_src) (st_tgt0, k_tgt x)>>),
             P i_src0 i_tgt0 w0 (st_src0, i_src)
               (st_tgt0, trigger (Choose X) >>= k_tgt))
         (TAKESRC: forall
-            i_src0 i_tgt0 w0 (st_src0: st_src) (st_tgt0: st_tgt)
+            i_src0 i_tgt0 w0 (st_src0: st_local) (st_tgt0: st_local)
             X k_src i_tgt
-            (K: forall (x: X), <<SIM: paco11 _sim_itree bot11 _ _ _ _ wf RR true i_tgt0 w0 (st_src0, k_src x) (st_tgt0, i_tgt)>> /\ <<IH: P true i_tgt0 w0 (st_src0, k_src x) (st_tgt0, i_tgt)>>),
+            (K: forall (x: X), <<SIM: paco8 _sim_itree bot8 _ _ RR true i_tgt0 w0 (st_src0, k_src x) (st_tgt0, i_tgt)>> /\ <<IH: P true i_tgt0 w0 (st_src0, k_src x) (st_tgt0, i_tgt)>>),
             P i_src0 i_tgt0 w0 (st_src0, trigger (Take X) >>= k_src)
               (st_tgt0, i_tgt))
         (TAKETGT: forall
-            i_src0 i_tgt0 w0 (st_src0: st_src) (st_tgt0: st_tgt)
+            i_src0 i_tgt0 w0 (st_src0: st_local) (st_tgt0: st_local)
             X i_src k_tgt
-            (K: exists (x: X), <<SIM:paco11 _sim_itree bot11 _ _ _ _ wf RR i_src0 true w0 (st_src0, i_src) (st_tgt0, k_tgt x)>> /\ <<IH: P i_src0 true w0 (st_src0, i_src) (st_tgt0, k_tgt x)>>),
+            (K: exists (x: X), <<SIM:paco8 _sim_itree bot8 _ _ RR i_src0 true w0 (st_src0, i_src) (st_tgt0, k_tgt x)>> /\ <<IH: P i_src0 true w0 (st_src0, i_src) (st_tgt0, k_tgt x)>>),
             P i_src0 i_tgt0 w0 (st_src0, i_src)
               (st_tgt0, trigger (Take X) >>= k_tgt))
         (SUPDATESRC: forall
-            i_src0 i_tgt0 w0 (st_src0: st_src) (st_tgt0: st_tgt)
+            i_src0 i_tgt0 w0 (st_src0: st_local) (st_tgt0: st_local)
             X k_src i_tgt
-            (run: st_src -> st_src * X )
-            (K: paco11 _sim_itree bot11 _ _ _ _ wf RR true i_tgt0 w0 (fst (run st_src0), k_src (snd (run st_src0))) (st_tgt0, i_tgt))
+            (run: st_local -> st_local * X )
+            (K: paco8 _sim_itree bot8 _ _ RR true i_tgt0 w0 (fst (run st_src0), k_src (snd (run st_src0))) (st_tgt0, i_tgt))
             (IH: P true i_tgt0 w0 (fst (run st_src0), k_src (snd (run st_src0))) (st_tgt0, i_tgt)),
             P i_src0 i_tgt0 w0 (st_src0, trigger (SUpdate run) >>= k_src) (st_tgt0, i_tgt))
         (SUPDATETGT: forall
-            i_src0 i_tgt0 w0 (st_src0: st_src) (st_tgt0: st_tgt)
+            i_src0 i_tgt0 w0 (st_src0: st_local) (st_tgt0: st_local)
             X i_src k_tgt
-            (run: st_tgt -> st_tgt * X )
-            (K: paco11 _sim_itree bot11 _ _ _ _ wf RR i_src0 true w0 (st_src0, i_src) (fst (run st_tgt0), k_tgt (snd (run st_tgt0))))
+            (run: st_local -> st_local * X )
+            (K: paco8 _sim_itree bot8 _ _ RR i_src0 true w0 (st_src0, i_src) (fst (run st_tgt0), k_tgt (snd (run st_tgt0))))
             (IH:  P i_src0 true w0 (st_src0, i_src) (fst (run st_tgt0), k_tgt (snd (run st_tgt0)))),
 
             P i_src0 i_tgt0 w0 (st_src0, i_src) (st_tgt0, trigger (SUpdate run) >>= k_tgt))       
         (PROGRESS: forall
-            i_src0 i_tgt0 w0 (st_src0: st_src) (st_tgt0: st_tgt)
+            i_src0 i_tgt0 w0 (st_src0: st_local) (st_tgt0: st_local)
             i_src i_tgt
-            (SIM: paco11 _sim_itree bot11 _ _ _ _ wf RR false false w0 (st_src0, i_src) (st_tgt0, i_tgt))
+            (SIM: paco8 _sim_itree bot8 _ _ RR false false w0 (st_src0, i_src) (st_tgt0, i_tgt))
             (SRC: i_src0 = true)
             (TGT: i_tgt0 = true),
             P true true w0 (st_src0, i_src) (st_tgt0, i_tgt))
     :
       forall i_src0 i_tgt0 w0 st_src st_tgt
-             (SIM: paco11 _sim_itree bot11 _ _ _ _ wf RR i_src0 i_tgt0 w0 st_src st_tgt),
+             (SIM: paco8 _sim_itree bot8 _ _ RR i_src0 i_tgt0 w0 st_src st_tgt),
         P i_src0 i_tgt0 w0 st_src st_tgt.
   Proof.
     i. punfold SIM. induction SIM using _sim_itree_ind2.
@@ -365,209 +365,209 @@ Section SIM.
 
   Qed.
 
-  Variant sim_itree_indC (sim_itree: forall (st_src st_tgt R_src R_tgt: Type) (wf: world -> st_src * st_tgt -> Prop) (RR: st_src -> st_tgt -> R_src -> R_tgt -> Prop), bool -> bool -> world -> st_src * itree (Es st_src) R_src -> st_tgt * itree (Es st_tgt) R_tgt -> Prop)
-          {st_src st_tgt R_src R_tgt} (wf: world -> (st_src * st_tgt) -> Prop) (RR: st_src -> st_tgt -> R_src -> R_tgt -> Prop)
-    : bool -> bool -> world -> st_src * itree (Es st_src) R_src -> st_tgt * itree (Es st_tgt) R_tgt -> Prop :=
+  Variant sim_itree_indC (sim_itree: forall (R_src R_tgt: Type) (RR: st_local -> st_local -> R_src -> R_tgt -> Prop), bool -> bool -> world -> st_local * itree Es R_src -> st_local * itree Es R_tgt -> Prop)
+          {R_src R_tgt} (RR: st_local -> st_local -> R_src -> R_tgt -> Prop)
+    : bool -> bool -> world -> st_local * itree Es R_src -> st_local * itree Es R_tgt -> Prop :=
   | sim_itree_indC_ret
       i_src0 i_tgt0 w0 st_src0 st_tgt0
       v_src v_tgt
       (RET: RR st_src0 st_tgt0 v_src v_tgt)
     :
-      sim_itree_indC sim_itree wf RR i_src0 i_tgt0 w0 (st_src0, Ret v_src) (st_tgt0, Ret v_tgt)
+      sim_itree_indC  sim_itree RR i_src0 i_tgt0 w0 (st_src0, Ret v_src) (st_tgt0, Ret v_tgt)
   | sim_itree_indC_call
       i_src0 i_tgt0 w w0 st_src0 st_tgt0
       fn varg k_src k_tgt
       (WF: wf w0 (st_src0, st_tgt0))
       (K: forall w1 vret st_src1 st_tgt1 (WLE: le w0 w1) (WF: wf w1 (st_src1, st_tgt1)),
-          sim_itree _ _ _ _ wf RR false false w (st_src1, k_src vret) (st_tgt1, k_tgt vret))
+          sim_itree _ _ RR false false w (st_src1, k_src vret) (st_tgt1, k_tgt vret))
     :
-      sim_itree_indC sim_itree wf RR i_src0 i_tgt0 w (st_src0, trigger (Call fn varg) >>= k_src)
+      sim_itree_indC  sim_itree RR i_src0 i_tgt0 w (st_src0, trigger (Call fn varg) >>= k_src)
                      (st_tgt0, trigger (Call fn varg) >>= k_tgt)
   | sim_itree_indC_syscall
-      i_src0 i_tgt0 w0 (st_src0: st_src) (st_tgt0: st_tgt)
+      i_src0 i_tgt0 w0 (st_src0: st_local) (st_tgt0: st_local)
       fn varg rvs k_src k_tgt
       (K: forall vret,
-          sim_itree _ _ _ _ wf RR true true w0 (st_src0, k_src vret) (st_tgt0, k_tgt vret))
+          sim_itree _ _ RR true true w0 (st_src0, k_src vret) (st_tgt0, k_tgt vret))
     :
-      sim_itree_indC sim_itree wf RR i_src0 i_tgt0 w0 (st_src0, trigger (Syscall fn varg rvs) >>= k_src)
+      sim_itree_indC  sim_itree RR i_src0 i_tgt0 w0 (st_src0, trigger (Syscall fn varg rvs) >>= k_src)
                      (st_tgt0, trigger (Syscall fn varg rvs) >>= k_tgt)
 
   | sim_itree_indC_tau_src
-      i_src0 i_tgt0 w0 (st_src0: st_src) (st_tgt0: st_tgt)
+      i_src0 i_tgt0 w0 (st_src0: st_local) (st_tgt0: st_local)
       i_src i_tgt
-      (K: sim_itree _ _ _ _ wf RR true i_tgt0 w0 (st_src0, i_src) (st_tgt0, i_tgt))
+      (K: sim_itree _ _ RR true i_tgt0 w0 (st_src0, i_src) (st_tgt0, i_tgt))
     :
-      sim_itree_indC sim_itree wf RR i_src0 i_tgt0 w0 (st_src0, tau;; i_src) (st_tgt0, i_tgt)
+      sim_itree_indC  sim_itree RR i_src0 i_tgt0 w0 (st_src0, tau;; i_src) (st_tgt0, i_tgt)
 
   | sim_itree_indC_tau_tgt
-      i_src0 i_tgt0 w0 (st_src0: st_src) (st_tgt0: st_tgt)
+      i_src0 i_tgt0 w0 (st_src0: st_local) (st_tgt0: st_local)
       i_src i_tgt
-      (K: sim_itree _ _ _ _ wf RR i_src0 true w0 (st_src0, i_src) (st_tgt0, i_tgt))
+      (K: sim_itree _ _ RR i_src0 true w0 (st_src0, i_src) (st_tgt0, i_tgt))
     :
-      sim_itree_indC sim_itree wf RR i_src0 i_tgt0 w0 (st_src0, i_src) (st_tgt0, tau;; i_tgt)
+      sim_itree_indC  sim_itree RR i_src0 i_tgt0 w0 (st_src0, i_src) (st_tgt0, tau;; i_tgt)
 
   | sim_itree_indC_choose_src
-      i_src0 i_tgt0 w0 (st_src0: st_src) (st_tgt0: st_tgt)
+      i_src0 i_tgt0 w0 (st_src0: st_local) (st_tgt0: st_local)
       X k_src i_tgt
-      (K: exists (x: X), sim_itree _ _ _ _ wf RR true i_tgt0 w0 (st_src0, k_src x) (st_tgt0, i_tgt))
+      (K: exists (x: X), sim_itree _ _ RR true i_tgt0 w0 (st_src0, k_src x) (st_tgt0, i_tgt))
     :
-      sim_itree_indC sim_itree wf RR i_src0 i_tgt0 w0 (st_src0, trigger (Choose X) >>= k_src)
+      sim_itree_indC  sim_itree RR i_src0 i_tgt0 w0 (st_src0, trigger (Choose X) >>= k_src)
                      (st_tgt0, i_tgt)
   | sim_itree_indC_choose_tgt
-      i_src0 i_tgt0 w0 (st_src0: st_src) (st_tgt0: st_tgt)
+      i_src0 i_tgt0 w0 (st_src0: st_local) (st_tgt0: st_local)
       X i_src k_tgt
-      (K: forall (x: X), sim_itree _ _ _ _ wf RR i_src0 true w0 (st_src0, i_src) (st_tgt0, k_tgt x))
+      (K: forall (x: X), sim_itree _ _ RR i_src0 true w0 (st_src0, i_src) (st_tgt0, k_tgt x))
     :
-      sim_itree_indC sim_itree wf RR i_src0 i_tgt0 w0 (st_src0, i_src)
+      sim_itree_indC  sim_itree RR i_src0 i_tgt0 w0 (st_src0, i_src)
                      (st_tgt0, trigger (Choose X) >>= k_tgt)
 
   | sim_itree_indC_take_src
-      i_src0 i_tgt0 w0 (st_src0: st_src) (st_tgt0: st_tgt)
+      i_src0 i_tgt0 w0 (st_src0: st_local) (st_tgt0: st_local)
       X k_src i_tgt
-      (K: forall (x: X), sim_itree _ _ _ _ wf RR true i_tgt0 w0 (st_src0, k_src x) (st_tgt0, i_tgt))
+      (K: forall (x: X), sim_itree _ _ RR true i_tgt0 w0 (st_src0, k_src x) (st_tgt0, i_tgt))
     :
-      sim_itree_indC sim_itree wf RR i_src0 i_tgt0 w0 (st_src0, trigger (Take X) >>= k_src)
+      sim_itree_indC  sim_itree RR i_src0 i_tgt0 w0 (st_src0, trigger (Take X) >>= k_src)
                      (st_tgt0, i_tgt)
   | sim_itree_indC_take_tgt
-      i_src0 i_tgt0 w0 (st_src0: st_src) (st_tgt0: st_tgt)
+      i_src0 i_tgt0 w0 (st_src0: st_local) (st_tgt0: st_local)
       X i_src k_tgt
-      (K: exists (x: X), sim_itree _ _ _ _ wf RR i_src0 true w0 (st_src0, i_src) (st_tgt0, k_tgt x))
+      (K: exists (x: X), sim_itree _ _ RR i_src0 true w0 (st_src0, i_src) (st_tgt0, k_tgt x))
     :
-      sim_itree_indC sim_itree wf RR i_src0 i_tgt0 w0 (st_src0, i_src)
+      sim_itree_indC  sim_itree RR i_src0 i_tgt0 w0 (st_src0, i_src)
                      (st_tgt0, trigger (Take X) >>= k_tgt)
   
   | sim_itree_indC_supdate_src
-      i_src0 i_tgt0 w0 (st_src0: st_src) (st_tgt0: st_tgt)
+      i_src0 i_tgt0 w0 (st_src0: st_local) (st_tgt0: st_local)
       X k_src i_tgt
-      (run: st_src -> st_src * X )
-      (K: sim_itree _ _ _ _ wf RR true i_tgt0 w0 (fst (run st_src0), k_src (snd (run st_src0))) (st_tgt0, i_tgt))
+      (run: st_local -> st_local * X )
+      (K: sim_itree _ _ RR true i_tgt0 w0 (fst (run st_src0), k_src (snd (run st_src0))) (st_tgt0, i_tgt))
     :
-      sim_itree_indC sim_itree wf RR i_src0 i_tgt0 w0 (st_src0, trigger (SUpdate run) >>= k_src) (st_tgt0, i_tgt)
+      sim_itree_indC  sim_itree RR i_src0 i_tgt0 w0 (st_src0, trigger (SUpdate run) >>= k_src) (st_tgt0, i_tgt)
 
   | sim_itree_indC_supdate_tgt
-      i_src0 i_tgt0 w0 (st_src0: st_src) (st_tgt0: st_tgt)
+      i_src0 i_tgt0 w0 (st_src0: st_local) (st_tgt0: st_local)
       X i_src k_tgt
-      (run: st_tgt -> st_tgt * X )
-      (K: sim_itree _ _ _ _ wf RR i_src0 true w0 (st_src0, i_src) (fst (run st_tgt0), k_tgt (snd (run st_tgt0))))
+      (run: st_local -> st_local * X )
+      (K: sim_itree _ _ RR i_src0 true w0 (st_src0, i_src) (fst (run st_tgt0), k_tgt (snd (run st_tgt0))))
     :
-      sim_itree_indC sim_itree wf RR i_src0 i_tgt0 w0 (st_src0, i_src) (st_tgt0, trigger (SUpdate run) >>= k_tgt)
+      sim_itree_indC  sim_itree RR i_src0 i_tgt0 w0 (st_src0, i_src) (st_tgt0, trigger (SUpdate run) >>= k_tgt)
   .
 
-  Lemma sim_itree_indC_mon: monotone11 sim_itree_indC.
+  Lemma sim_itree_indC_mon: monotone8 sim_itree_indC.
   Proof.
     ii. inv IN; try (by des; econs; ss; et).
   Qed.
   Hint Resolve sim_itree_indC_mon: paco.
 
   Lemma sim_itree_indC_spec:
-    sim_itree_indC <12= gupaco11 (_sim_itree) (cpn11 _sim_itree).
+    sim_itree_indC <9= gupaco8 (_sim_itree) (cpn8 _sim_itree).
   Proof.
-    eapply wrespect11_uclo; eauto with paco.
+    eapply wrespect8_uclo; eauto with paco.
     econs; eauto with paco. i. inv PR.
     { econs 1; eauto. }
     { econs 2; eauto. i. exploit K; eauto. i. des.
-      esplits; eauto. eapply rclo11_base. eauto. }
-    { econs 3; eauto. i. eapply rclo11_base. eauto. }
-    { econs 4; eauto. eapply sim_itree_mon; eauto. i. eapply rclo11_base. eauto. }
-    { econs 5; eauto. eapply sim_itree_mon; eauto. i. eapply rclo11_base. eauto. }
-    { econs 6; eauto. des. esplits; eauto. eapply sim_itree_mon; eauto. i. eapply rclo11_base. eauto. }
-    { econs 7; eauto. i. eapply sim_itree_mon; eauto. i. eapply rclo11_base. eauto. }
-    { econs 8; eauto. i. eapply sim_itree_mon; eauto. i. eapply rclo11_base. eauto. }
-    { econs 9; eauto. des. esplits; eauto. eapply sim_itree_mon; eauto. i. eapply rclo11_base. eauto. }
-    { econs 10; eauto. des. esplits; eauto. eapply sim_itree_mon; eauto. i. eapply rclo11_base. eauto.  }
-    { econs 11; eauto. des. esplits; eauto.  eapply sim_itree_mon; eauto. i. eapply rclo11_base. eauto.  }
+      esplits; eauto. eapply rclo8_base. eauto. }
+    { econs 3; eauto. i. eapply rclo8_base. eauto. }
+    { econs 4; eauto. eapply sim_itree_mon; eauto. i. eapply rclo8_base. eauto. }
+    { econs 5; eauto. eapply sim_itree_mon; eauto. i. eapply rclo8_base. eauto. }
+    { econs 6; eauto. des. esplits; eauto. eapply sim_itree_mon; eauto. i. eapply rclo8_base. eauto. }
+    { econs 7; eauto. i. eapply sim_itree_mon; eauto. i. eapply rclo8_base. eauto. }
+    { econs 8; eauto. i. eapply sim_itree_mon; eauto. i. eapply rclo8_base. eauto. }
+    { econs 9; eauto. des. esplits; eauto. eapply sim_itree_mon; eauto. i. eapply rclo8_base. eauto. }
+    { econs 10; eauto. des. esplits; eauto. eapply sim_itree_mon; eauto. i. eapply rclo8_base. eauto.  }
+    { econs 11; eauto. des. esplits; eauto.  eapply sim_itree_mon; eauto. i. eapply rclo8_base. eauto.  }
   Qed.
 
-  Variant sim_itreeC (r g: forall (st_src st_tgt R_src R_tgt: Type) (wf: world -> (st_src * st_tgt) -> Prop) (RR: st_src -> st_tgt -> R_src -> R_tgt -> Prop), bool -> bool -> world -> st_src * itree (Es st_src) R_src -> st_tgt * itree (Es st_tgt) R_tgt -> Prop)
-          {st_src st_tgt R_src R_tgt} (wf: world -> st_src * st_tgt -> Prop) (RR: st_src -> st_tgt -> R_src -> R_tgt -> Prop)
-    : bool -> bool -> world -> st_src * itree (Es st_src) R_src -> st_tgt * itree (Es st_tgt) R_tgt -> Prop :=
+  Variant sim_itreeC (r g: forall (R_src R_tgt: Type) (RR: st_local -> st_local -> R_src -> R_tgt -> Prop), bool -> bool -> world -> st_local * itree Es R_src -> st_local * itree Es R_tgt -> Prop)
+          {R_src R_tgt} (RR: st_local -> st_local -> R_src -> R_tgt -> Prop)
+    : bool -> bool -> world -> st_local * itree Es R_src -> st_local * itree Es R_tgt -> Prop :=
   | sim_itreeC_ret
       i_src0 i_tgt0 w0 st_src0 st_tgt0
       v_src v_tgt
       (RET: RR st_src0 st_tgt0 v_src v_tgt)
     :
-      sim_itreeC r g wf RR i_src0 i_tgt0 w0 (st_src0, Ret v_src) (st_tgt0, Ret v_tgt)
+      sim_itreeC r g RR i_src0 i_tgt0 w0 (st_src0, Ret v_src) (st_tgt0, Ret v_tgt)
   | sim_itreeC_call
       i_src0 i_tgt0 w w0 st_src0 st_tgt0
       fn varg k_src k_tgt
       (WF: wf w0 (st_src0, st_tgt0))
       (K: forall w1 vret st_src1 st_tgt1 (WLE: le w0 w1) (WF: wf w1 (st_src1, st_tgt1)),
-          g _ _ _ _ wf RR false false w (st_src1, k_src vret) (st_tgt1, k_tgt vret))
+          g _ _ RR false false w (st_src1, k_src vret) (st_tgt1, k_tgt vret))
     :
-      sim_itreeC r g wf RR i_src0 i_tgt0 w (st_src0, trigger (Call fn varg) >>= k_src)
+      sim_itreeC r g RR i_src0 i_tgt0 w (st_src0, trigger (Call fn varg) >>= k_src)
                  (st_tgt0, trigger (Call fn varg) >>= k_tgt)
   | sim_itreeC_syscall
-      i_src0 i_tgt0 w0 (st_src0: st_src) (st_tgt0: st_tgt)
+      i_src0 i_tgt0 w0 (st_src0: st_local) (st_tgt0: st_local)
       fn varg rvs k_src k_tgt
       (K: forall vret,
-          g _ _ _ _ wf RR true true w0 (st_src0, k_src vret) (st_tgt0, k_tgt vret))
+          g _ _ RR true true w0 (st_src0, k_src vret) (st_tgt0, k_tgt vret))
     :
-      sim_itreeC r g wf RR i_src0 i_tgt0 w0 (st_src0, trigger (Syscall fn varg rvs) >>= k_src)
+      sim_itreeC r g RR i_src0 i_tgt0 w0 (st_src0, trigger (Syscall fn varg rvs) >>= k_src)
                  (st_tgt0, trigger (Syscall fn varg rvs) >>= k_tgt)
 
   | sim_itreeC_tau_src
-      i_src0 i_tgt0 w0 (st_src0: st_src) (st_tgt0: st_tgt)
+      i_src0 i_tgt0 w0 (st_src0: st_local) (st_tgt0: st_local)
       i_src i_tgt
-      (K: r _ _ _ _ wf RR true i_tgt0 w0 (st_src0, i_src) (st_tgt0, i_tgt))
+      (K: r _ _ RR true i_tgt0 w0 (st_src0, i_src) (st_tgt0, i_tgt))
     :
-      sim_itreeC r g wf RR i_src0 i_tgt0 w0 (st_src0, tau;; i_src) (st_tgt0, i_tgt)
+      sim_itreeC r g RR i_src0 i_tgt0 w0 (st_src0, tau;; i_src) (st_tgt0, i_tgt)
 
   | sim_itreeC_tau_tgt
-      i_src0 i_tgt0 w0 (st_src0: st_src) (st_tgt0: st_tgt)
+      i_src0 i_tgt0 w0 (st_src0: st_local) (st_tgt0: st_local)
       i_src i_tgt
-      (K: r _ _ _ _ wf RR i_src0 true w0 (st_src0, i_src) (st_tgt0, i_tgt))
+      (K: r _ _ RR i_src0 true w0 (st_src0, i_src) (st_tgt0, i_tgt))
     :
-      sim_itreeC r g wf RR i_src0 i_tgt0 w0 (st_src0, i_src) (st_tgt0, tau;; i_tgt)
+      sim_itreeC r g RR i_src0 i_tgt0 w0 (st_src0, i_src) (st_tgt0, tau;; i_tgt)
 
 
   | sim_itreeC_choose_src
-      i_src0 i_tgt0 w0 (st_src0: st_src) (st_tgt0: st_tgt)
+      i_src0 i_tgt0 w0 (st_src0: st_local) (st_tgt0: st_local)
       X k_src i_tgt
-      (K: exists (x: X), r _ _ _ _ wf RR true i_tgt0 w0 (st_src0, k_src x) (st_tgt0, i_tgt))
+      (K: exists (x: X), r _ _ RR true i_tgt0 w0 (st_src0, k_src x) (st_tgt0, i_tgt))
     :
-      sim_itreeC r g wf RR i_src0 i_tgt0 w0 (st_src0, trigger (Choose X) >>= k_src)
+      sim_itreeC r g RR i_src0 i_tgt0 w0 (st_src0, trigger (Choose X) >>= k_src)
                  (st_tgt0, i_tgt)
   | sim_itreeC_choose_tgt
-      i_src0 i_tgt0 w0 (st_src0: st_src) (st_tgt0: st_tgt)
+      i_src0 i_tgt0 w0 (st_src0: st_local) (st_tgt0: st_local)
       X i_src k_tgt
-      (K: forall (x: X), r _ _ _ _ wf RR i_src0 true w0 (st_src0, i_src) (st_tgt0, k_tgt x))
+      (K: forall (x: X), r _ _ RR i_src0 true w0 (st_src0, i_src) (st_tgt0, k_tgt x))
     :
-      sim_itreeC r g wf RR i_src0 i_tgt0 w0 (st_src0, i_src)
+      sim_itreeC r g RR i_src0 i_tgt0 w0 (st_src0, i_src)
                  (st_tgt0, trigger (Choose X) >>= k_tgt)
   | sim_itreeC_take_src
-      i_src0 i_tgt0 w0 (st_src0: st_src) (st_tgt0: st_tgt)
+      i_src0 i_tgt0 w0 (st_src0: st_local) (st_tgt0: st_local)
       X k_src i_tgt
-      (K: forall (x: X), r _ _ _ _ wf RR true i_tgt0 w0 (st_src0, k_src x) (st_tgt0, i_tgt))
+      (K: forall (x: X), r _ _ RR true i_tgt0 w0 (st_src0, k_src x) (st_tgt0, i_tgt))
     :
-      sim_itreeC r g wf RR i_src0 i_tgt0 w0 (st_src0, trigger (Take X) >>= k_src)
+      sim_itreeC r g RR i_src0 i_tgt0 w0 (st_src0, trigger (Take X) >>= k_src)
                  (st_tgt0, i_tgt)
   | sim_itreeC_take_tgt
-      i_src0 i_tgt0 w0 (st_src0: st_src) (st_tgt0: st_tgt)
+      i_src0 i_tgt0 w0 (st_src0: st_local) (st_tgt0: st_local)
       X i_src k_tgt
-      (K: exists (x: X), r _ _ _ _ wf RR i_src0 true w0 (st_src0, i_src) (st_tgt0, k_tgt x))
+      (K: exists (x: X), r _ _ RR i_src0 true w0 (st_src0, i_src) (st_tgt0, k_tgt x))
     :
-      sim_itreeC r g wf RR i_src0 i_tgt0 w0 (st_src0, i_src)
+      sim_itreeC r g RR i_src0 i_tgt0 w0 (st_src0, i_src)
                  (st_tgt0, trigger (Take X) >>= k_tgt)
   | sim_itreeC_supdate_src
-      i_src0 i_tgt0 w0 (st_src0: st_src) (st_tgt0: st_tgt)
+      i_src0 i_tgt0 w0 (st_src0: st_local) (st_tgt0: st_local)
       X k_src i_tgt
-      (run: st_src -> st_src * X )
-      (K: r _ _ _ _ wf RR true i_tgt0 w0 (fst (run st_src0), k_src (snd (run st_src0))) (st_tgt0, i_tgt))
+      (run: st_local -> st_local * X )
+      (K: r _ _ RR true i_tgt0 w0 (fst (run st_src0), k_src (snd (run st_src0))) (st_tgt0, i_tgt))
     :
-      sim_itreeC r g wf RR i_src0 i_tgt0 w0 (st_src0, trigger (SUpdate run) >>= k_src) (st_tgt0, i_tgt)
+      sim_itreeC r g RR i_src0 i_tgt0 w0 (st_src0, trigger (SUpdate run) >>= k_src) (st_tgt0, i_tgt)
 
   | sim_itreeC_supdate_tgt
-      i_src0 i_tgt0 w0 (st_src0: st_src) (st_tgt0: st_tgt)
+      i_src0 i_tgt0 w0 (st_src0: st_local) (st_tgt0: st_local)
       X i_src k_tgt
-      (run: st_tgt -> st_tgt * X )
-      (K: r _ _ _ _ wf RR i_src0 true w0 (st_src0, i_src) (fst (run st_tgt0), k_tgt (snd (run st_tgt0))))
+      (run: st_local -> st_local * X )
+      (K: r _ _ RR i_src0 true w0 (st_src0, i_src) (fst (run st_tgt0), k_tgt (snd (run st_tgt0))))
     :
-      sim_itreeC r g wf RR i_src0 i_tgt0 w0 (st_src0, i_src) (st_tgt0, trigger (SUpdate run) >>= k_tgt)
+      sim_itreeC r g RR i_src0 i_tgt0 w0 (st_src0, i_src) (st_tgt0, trigger (SUpdate run) >>= k_tgt)
 
   .
 
   Lemma sim_itreeC_spec_aux:
-    sim_itreeC <13= gpaco11 (_sim_itree) (cpn11 _sim_itree).
+    sim_itreeC <10= gpaco8 (_sim_itree) (cpn8 _sim_itree).
   Proof.
     i. inv PR.
     { gstep. econs 1; eauto. }
@@ -585,35 +585,35 @@ Section SIM.
 
   Lemma sim_itreeC_spec r g
     :
-      @sim_itreeC (gpaco11 (_sim_itree) (cpn11 _sim_itree) r g) (gpaco11 (_sim_itree) (cpn11 _sim_itree) g g)
-      <11=
-      gpaco11 (_sim_itree) (cpn11 _sim_itree) r g.
+      @sim_itreeC (gpaco8 (_sim_itree) (cpn8 _sim_itree) r g) (gpaco8 (_sim_itree) (cpn8 _sim_itree) g g)
+      <8=
+      gpaco8 (_sim_itree) (cpn8 _sim_itree) r g.
   Proof.
-    i. eapply gpaco11_gpaco; [eauto with paco|].
-    eapply gpaco11_mon.
+    i. eapply gpaco8_gpaco; [eauto with paco|].
+    eapply gpaco8_mon.
     { eapply sim_itreeC_spec_aux. eauto. }
     { auto. }
-    { i. eapply gupaco11_mon; eauto. }
+    { i. eapply gupaco8_mon; eauto. }
   Qed.
 
-  Lemma sim_itree_progress_flag {st_src st_tgt} R0 R1 (wf: world -> (st_src * st_tgt) -> Prop) RR w r g st_src0 st_tgt0
-        (SIM: gpaco11 _sim_itree (cpn11 _sim_itree) g g _ _ R0 R1 wf RR false false w st_src0 st_tgt0)
+  Lemma sim_itree_progress_flag R0 R1 RR w r g st_src0 st_tgt0
+        (SIM: gpaco8 _sim_itree (cpn8 _sim_itree) g g R0 R1 RR false false w st_src0 st_tgt0)
     :
-      gpaco11 _sim_itree (cpn11 _sim_itree) r g _ _ R0 R1 wf RR true true w st_src0 st_tgt0.
+      gpaco8 _sim_itree (cpn8 _sim_itree) r g R0 R1 RR true true w st_src0 st_tgt0.
   Proof.
     gstep. destruct st_src0, st_tgt0. econs; eauto. 
   Qed.
 
   Lemma sim_itree_flag_mon
-        (sim_itree: forall (st_src st_tgt R_src R_tgt: Type) (wf: world -> st_src * st_tgt -> Prop)
-                           (RR: st_src -> st_tgt -> R_src -> R_tgt -> Prop), bool -> bool -> world -> st_src * itree (Es st_src) R_src -> st_tgt * itree (Es st_tgt) R_tgt -> Prop)
-        {st_src st_tgt} R_src R_tgt (wf: world -> st_src * st_tgt -> Prop) (RR: st_src -> st_tgt -> R_src -> R_tgt -> Prop)
+        (sim_itree: forall (R_src R_tgt: Type)
+                           (RR: st_local -> st_local -> R_src -> R_tgt -> Prop), bool -> bool -> world -> st_local * itree Es R_src -> st_local * itree Es R_tgt -> Prop)
+        R_src R_tgt (RR: st_local -> st_local -> R_src -> R_tgt -> Prop)
         f_src0 f_tgt0 f_src1 f_tgt1 w st_src0 st_tgt0
-        (SIM: @_sim_itree sim_itree _ _ _ _  wf RR f_src0 f_tgt0 w st_src0 st_tgt0)
+        (SIM: @_sim_itree sim_itree _ _ RR f_src0 f_tgt0 w st_src0 st_tgt0)
         (SRC: f_src0 = true -> f_src1 = true)
         (TGT: f_tgt0 = true -> f_tgt1 = true)
     :
-      @_sim_itree sim_itree _ _ _ _ wf RR f_src1 f_tgt1 w st_src0 st_tgt0.
+      @_sim_itree sim_itree _ _ RR f_src1 f_tgt1 w st_src0 st_tgt0.
   Proof.
     revert f_src1 f_tgt1 SRC TGT.
     induction SIM using _sim_itree_ind2; i; clarify.
@@ -631,68 +631,54 @@ Section SIM.
     { exploit SRC0; auto. exploit TGT0; auto. i. clarify. econs; eauto. }
   Qed.
 
-  Definition respectful' := 
-    fun (A B C D: Type) (R: A -> B -> Prop) (R': C -> D -> Prop) (f: A -> C) (g: B -> D) 
-    => forall x y, R x y -> R' (f x) (g y).
 
-  Definition sim_fsem {st_src st_tgt} (wf: world -> st_src * st_tgt -> Prop): 
-  (Any.t -> itree (Es st_src) Any.t) -> (Any.t -> itree (Es st_tgt) Any.t) -> Prop :=
-    (respectful' eq (fun it_src it_tgt => forall w mrs_src mrs_tgt
-    (SIMMRS: wf w (mrs_src, mrs_tgt)), 
-    sim_itree false false w wf (mrs_src, it_src) (mrs_tgt, it_tgt)
-    ))%signature.
-
-
-  (* Definition sim_fsem: relation (option mname * Any.t -> itree (Es st) Any.t) :=
+  Definition sim_fsem: relation ( Any.t -> itree Es Any.t) :=
     (eq ==> (fun it_src it_tgt => forall w mrs_src mrs_tgt (SIMMRS: wf w (mrs_src, mrs_tgt)),
                  sim_itree false false w (mrs_src, it_src)
                            (mrs_tgt, it_tgt)))%signature
-  . *)
+  .
 
-  Definition sim_fnsem {st_src st_tgt} (wf: world -> st_src * st_tgt -> Prop): (gname -> option (Any.t -> itree (Es st_src) Any.t)) -> (gname -> option (Any.t -> itree (Es st_tgt) Any.t)) -> Prop :=
-    fun f g => forall s, match (f s), (g s) with
-                        | Some x, Some y => sim_fsem wf x y
+  Definition sim_fnsem: relation (gname -> option (Any.t -> itree Es Any.t)) := 
+   fun f g => forall s, match (f s), (g s) with
+                        | Some x, Some y => sim_fsem x y
                         | None, None => True
                         | _, _ => False
                         end
     .
 
-  (* Definition sim_fnsem: relation (string * (option mname * Any.t -> itree (Es st) Any.t)) := RelProd eq sim_fsem. *)
-
-
-  Variant lflagC (r: forall (st_src st_tgt R_src R_tgt: Type) (wf: world -> st_src * st_tgt -> Prop)
-    (RR: st_src -> st_tgt -> R_src -> R_tgt -> Prop), bool -> bool -> world -> st_src * itree (Es st_src) R_src -> st_tgt * itree (Es st_tgt) R_tgt -> Prop)
-          {st_src st_tgt R_src R_tgt} (wf: world -> st_src * st_tgt -> Prop) (RR: st_src -> st_tgt -> R_src -> R_tgt -> Prop)
-    : bool -> bool -> world -> st_src * itree (Es st_src) R_src -> st_tgt * itree (Es st_tgt) R_tgt -> Prop :=
+  Variant lflagC (r: forall (R_src R_tgt: Type)
+    (RR: st_local -> st_local -> R_src -> R_tgt -> Prop), bool -> bool -> world -> st_local * itree Es R_src -> st_local * itree Es R_tgt -> Prop)
+          {R_src R_tgt} (RR: st_local -> st_local -> R_src -> R_tgt -> Prop)
+    : bool -> bool -> world -> st_local * itree Es R_src -> st_local * itree Es R_tgt -> Prop :=
   | lflagC_intro
       f_src0 f_src1 f_tgt0 f_tgt1 w st_src st_tgt
-      (SIM: r _ _ _ _ wf RR f_src0 f_tgt0 w st_src st_tgt)
+      (SIM: r _ _ RR f_src0 f_tgt0 w st_src st_tgt)
       (SRC: f_src0 = true -> f_src1 = true)
       (TGT: f_tgt0 = true -> f_tgt1 = true)
     :
-      lflagC r wf RR f_src1 f_tgt1 w st_src st_tgt
+      lflagC r RR f_src1 f_tgt1 w st_src st_tgt
   .
 
   Lemma lflagC_mon
         r1 r2
-        (LE: r1 <11= r2)
+        (LE: r1  <8= r2)
     :
-      @lflagC r1 <11= @lflagC r2
+      @lflagC r1  <8= @lflagC r2
   .
   Proof. ii. destruct PR; econs; et. Qed.
 
   Hint Resolve lflagC_mon: paco.
 
-  Lemma lflagC_spec: lflagC <12= gupaco11 (_sim_itree) (cpn11 _sim_itree).
+  Lemma lflagC_spec: lflagC  <9= gupaco8 (_sim_itree) (cpn8 _sim_itree).
   Proof.
-    eapply wrespect11_uclo; eauto with paco.
+    eapply wrespect8_uclo; eauto with paco.
     econs; eauto with paco. i. inv PR.
     eapply GF in SIM.
-    revert x6 x7 SRC TGT. induction SIM using _sim_itree_ind2; i; clarify.
+    revert x3 x4 SRC TGT. induction SIM using _sim_itree_ind2; i; clarify.
     { econs 1; eauto. }
     { econs 2; eauto. i. exploit K; eauto. i. des.
-      esplits; eauto. eapply rclo11_base. eauto. }
-    { econs 3; eauto. i. eapply rclo11_base. eauto. }
+      esplits; eauto. eapply rclo8_base. eauto. }
+    { econs 3; eauto. i. eapply rclo8_base. eauto. }
     { econs 4; eauto. }
     { econs 5; eauto. }
     { econs 6; eauto.  des. esplits; eauto. }
@@ -702,21 +688,21 @@ Section SIM.
     { econs 10; eauto. }
     { econs 11; eauto. }
     { exploit SRC0; auto. exploit TGT0; auto. i. clarify. econs 12; eauto.
-      eapply rclo11_base; auto. }
+      eapply rclo8_base; auto. }
   Qed.
 
-  Lemma sim_itree_flag_down {st_src st_tgt} R0 R1 (wf: world -> st_src * st_tgt -> Prop) RR r g w st_src0 st_tgt0 f_src f_tgt
-        (SIM: gpaco11 _sim_itree (cpn11 _sim_itree) r g _ _ R0 R1 wf RR false false w st_src0 st_tgt0)
+  Lemma sim_itree_flag_down  R0 R1 RR r g w st_src0 st_tgt0 f_src f_tgt
+        (SIM: gpaco8 _sim_itree (cpn8 _sim_itree) r g R0 R1 RR false false w st_src0 st_tgt0)
     :
-      gpaco11 _sim_itree (cpn11 _sim_itree) r g _ _ R0 R1 wf RR f_src f_tgt w st_src0 st_tgt0.
+      gpaco8 _sim_itree (cpn8 _sim_itree) r g R0 R1 RR f_src f_tgt w st_src0 st_tgt0.
   Proof.
     guclo lflagC_spec. econs; eauto.
   Qed.
 
-  Lemma sim_itree_bot_flag_up {st_src st_tgt} R0 R1 (wf: world -> st_src * st_tgt -> Prop) RR w st_src0 st_tgt0 f_src f_tgt
-        (SIM: paco11 _sim_itree bot11 _ _ R0 R1 wf RR true true w st_src0 st_tgt0)
+  Lemma sim_itree_bot_flag_up  R0 R1 RR w st_src0 st_tgt0 f_src f_tgt
+        (SIM: paco8 _sim_itree bot8 R0 R1 RR true true w st_src0 st_tgt0)
     :
-      paco11 _sim_itree bot11 _ _ R0 R1 wf RR f_src f_tgt w st_src0 st_tgt0.
+      paco8 _sim_itree bot8 R0 R1 RR f_src f_tgt w st_src0 st_tgt0.
   Proof.
     ginit. remember true in SIM at 1. remember true in SIM at 1.
     clear Heqb Heqb0. revert w st_src0 st_tgt0 f_src f_tgt b b0 SIM.
@@ -729,7 +715,7 @@ Section SIM.
     | |- ?P b b0 w st_src0 st_tgt0 => set P
     end.
     revert b b0 w st_src0 st_tgt0 SIM.
-    eapply (@sim_itree_ind _ _ R0 R1 wf RR P); subst P; ss; i; clarify.
+    eapply (@sim_itree_ind R0 R1 RR P); subst P; ss; i; clarify.
     { guclo sim_itree_indC_spec. econs 1; eauto. }
     { gstep. econs 2; eauto. i. gbase. eapply CIH; eauto. }
     { gstep. econs 3; eauto. i. gbase. eapply CIH; eauto. }
@@ -742,41 +728,40 @@ Section SIM.
     { guclo sim_itree_indC_spec. econs 10; eauto. } 
     { guclo sim_itree_indC_spec. econs 11; eauto. } 
     { eapply sim_itree_flag_down. gfinal. right.
-      eapply paco11_mon; eauto. ss.
+      eapply paco8_mon; eauto. ss.
     }
   Qed.
 
-  Variant lbindR (r s: forall st_src st_tgt S_src S_tgt (wf: world -> st_src * st_tgt -> Prop) (SS: st_src -> st_tgt -> S_src -> S_tgt -> Prop), bool -> bool -> world -> st_src * itree (Es st_src) S_src -> st_tgt * itree (Es st_tgt) S_tgt -> Prop):
-    forall st_src st_tgt S_src S_tgt (wf: world -> st_src * st_tgt -> Prop) (SS: st_src -> st_tgt -> S_src -> S_tgt -> Prop), bool -> bool -> world -> st_src * itree (Es st_src) S_src -> st_tgt * itree (Es st_tgt) S_tgt -> Prop :=
+  Variant lbindR (r s: forall S_src S_tgt (SS: st_local -> st_local -> S_src -> S_tgt -> Prop), bool -> bool -> world -> st_local * itree Es S_src -> st_local * itree Es S_tgt -> Prop):
+    forall S_src S_tgt (SS: st_local -> st_local -> S_src -> S_tgt -> Prop), bool -> bool -> world -> st_local * itree Es S_src -> st_local * itree Es S_tgt -> Prop :=
   | lbindR_intro
       f_src f_tgt w0 w1
-      st_src st_tgt
-      R_src R_tgt wf RR
-      (st_src0: st_src )(st_tgt0: st_tgt)
-      (i_src: itree (Es st_src) R_src) (i_tgt: itree (Es st_tgt) R_tgt)
-      (SIM: r _ _ _ _ wf RR f_src f_tgt w0 (st_src0, i_src) (st_tgt0, i_tgt))
+      R_src R_tgt RR
+      (st_src0 st_tgt0: st_local)
+      (i_src: itree Es R_src) (i_tgt: itree Es R_tgt)
+      (SIM: r _ _ RR f_src f_tgt w0 (st_src0, i_src) (st_tgt0, i_tgt))
 
       S_src S_tgt SS
-      (k_src: ktree (Es st_src) R_src S_src) (k_tgt: ktree (Es st_tgt) R_tgt S_tgt)
-      (SIMK: forall st_src1 st_tgt1 vret_src vret_tgt (SIM: RR st_src1 st_tgt1 vret_src vret_tgt), s _ _ _ _ wf SS false false w1 (st_src1, k_src vret_src) (st_tgt1, k_tgt vret_tgt))
+      (k_src: ktree Es R_src S_src) (k_tgt: ktree Es R_tgt S_tgt)
+      (SIMK: forall st_src1 st_tgt1 vret_src vret_tgt (SIM: RR st_src1 st_tgt1 vret_src vret_tgt), s _ _ SS false false w1 (st_src1, k_src vret_src) (st_tgt1, k_tgt vret_tgt))
     :
-      lbindR r s wf SS f_src f_tgt w1 (st_src0, ITree.bind i_src k_src) (st_tgt0, ITree.bind i_tgt k_tgt)
+      lbindR r s SS f_src f_tgt w1 (st_src0, ITree.bind i_src k_src) (st_tgt0, ITree.bind i_tgt k_tgt)
   .
 
   Hint Constructors lbindR: core.
 
   Lemma lbindR_mon 
         r1 r2 s1 s2
-        (LEr: r1 <11= r2) (LEs: s1 <11= s2)
+        (LEr: r1  <8= r2) (LEs: s1  <8= s2)
     :
-      lbindR r1 s1 <11= lbindR r2 s2
+      lbindR r1 s1  <8= lbindR r2 s2
   .
   Proof. ii. destruct PR; econs; et. Qed.
 
   Definition lbindC r := lbindR r r.
   Hint Unfold lbindC: core.
 
-  Lemma lbindC_wrespectful: wrespectful11 (_sim_itree) lbindC.
+  Lemma lbindC_wrespectful: wrespectful8 (_sim_itree) lbindC.
   Proof.
     econs.
     { ii. eapply lbindR_mon; eauto. }
@@ -787,13 +772,13 @@ Section SIM.
     induction SIM using _sim_itree_ind2; i; clarify.
     + rewrite ! bind_ret_l. exploit SIMK; eauto. i.
       eapply sim_itree_flag_mon.
-      { eapply sim_itree_mon; eauto. i. eapply rclo11_base. auto. }
+      { eapply sim_itree_mon; eauto. i. eapply rclo8_base. auto. }
       { ss. }
       { ss. }
     + rewrite ! bind_bind. econs; eauto. i.
-      eapply rclo11_clo_base. econs; eauto.
+      eapply rclo8_clo_base. econs; eauto.
     + rewrite ! bind_bind. econs; eauto. i.
-      eapply rclo11_clo_base. econs; eauto.
+      eapply rclo8_clo_base. econs; eauto.
     + rewrite ! bind_tau. econs; eauto.
     + rewrite ! bind_tau. econs; eauto.
     + rewrite ! bind_bind. econs; eauto. des. esplits; eauto.
@@ -802,21 +787,21 @@ Section SIM.
     + rewrite ! bind_bind. econs; eauto. des. esplits; eauto.
     + rewrite ! bind_bind. econs; eauto. 
     + rewrite ! bind_bind. econs; eauto. 
-    + econs; eauto. eapply rclo11_clo_base. econs; eauto.
+    + econs; eauto. eapply rclo8_clo_base. econs; eauto.
   Qed.
 
-  Lemma lbindC_spec: lbindC <12= gupaco11 (_sim_itree) (cpn11 (_sim_itree)).
+  Lemma lbindC_spec: lbindC  <9= gupaco8 (_sim_itree) (cpn8 (_sim_itree)).
   Proof.
-    intros. eapply wrespect11_uclo; eauto with paco. eapply lbindC_wrespectful.
+    intros. eapply wrespect8_uclo; eauto with paco. eapply lbindC_wrespectful.
   Qed.
 
 End SIM.
 Hint Resolve sim_itree_mon: paco.
-Hint Resolve cpn11_wcompat: paco.
+Hint Resolve cpn8_wcompat: paco.
 
 Lemma self_sim_itree:
-  forall w st st0 itr,
-    @sim_itree unit top2 st st false false w (fun _ '(src, tgt) => src = tgt) (st0, itr) (st0, itr).
+  forall st itr,
+    sim_itree (fun _ '(src, tgt) => src = tgt) top2 false false tt (st, itr) (st, itr).
 Proof.
   ginit. gcofix CIH. i. ides itr.
   { gstep. eapply sim_itree_ret; ss. }
@@ -863,14 +848,14 @@ Section SIMMODSEM.
 
   Variable (ms_src ms_tgt: ModSem.t).
 
-  Let W: Type := (ms_src.(ModSem.state)) * (ms_tgt.(ModSem.state)).
+  Let W: Type := (Any.t) * (Any.t).
 
   Inductive sim: Prop := mk {
     world: Type;
     wf: world -> W -> Prop;
     le: world -> world -> Prop;
     le_PreOrder: PreOrder le;
-    sim_fnsems: (sim_fnsem le wf) (ms_src.(ModSem.fnsems)) (ms_tgt.(ModSem.fnsems));
+    sim_fnsems: (sim_fnsem wf le) (ms_src.(ModSem.fnsems)) (ms_tgt.(ModSem.fnsems));
     (* sim_fnsems: Forall2 (sim_fnsem wf le) ms_src.(ModSem.fnsems) ms_tgt.(ModSem.fnsems); *)
     (* sim_mn: ms_src.(ModSem.mn) = ms_tgt.(ModSem.mn); *)
     sim_initial: exists w_init, wf w_init (ms_src.(ModSem.init_st), ms_tgt.(ModSem.init_st));
@@ -885,8 +870,8 @@ Proof.
   - instantiate (1:=fun (_ _: unit) => True). ss.
   - instantiate (1:=(fun (_: unit) '(src, tgt) => src = tgt)).
     unfold sim_fnsem. ii. des_ifs.
-    unfold sim_fsem, respectful'. ii. destruct H, SIMMRS.
-    apply self_sim_itree.  
+    unfold sim_fsem, respectful. ii. destruct H, SIMMRS.
+    rewrite w. apply self_sim_itree.  
   - ss.
 Qed.
 
@@ -923,15 +908,15 @@ Section SIMMOD.
 
   Lemma Mod_add_fnsems md0 md1 sk
     :
-      (ModSem.fnsems (Mod.get_modsem (Mod.add md0 md1) sk)) =
-      ModSem.add_fnsems (Mod.get_modsem md0 sk) (Mod.get_modsem md1 sk).
+      (ModSem.fnsems (Mod.get_modsem (ModAdd.add md0 md1) sk)) =
+      ModSemAdd.add_fnsems (Mod.get_modsem md0 sk) (Mod.get_modsem md1 sk).
   Proof.
     ss.
   Qed.
 
   Lemma Mod_add_sk md0 md1
     :
-      Mod.sk (Mod.add md0 md1) = Mod.sk md0 ++ Mod.sk md1.
+      Mod.sk (ModAdd.add md0 md1) = Mod.sk md0 ++ Mod.sk md1.
   Proof.
     ss.
   Qed.
@@ -983,9 +968,7 @@ Section ADEQUACY.
 
     (* Variable mn: mname. *)
     Variable world: Type.
-    Let W: Type := (ms_src.(ModSem.state)) * (ms_tgt.(ModSem.state)). 
-    Variable wf: world -> W -> Prop. 
-    (* Variable wf: world -> Any.t * Any.t -> Prop. *)
+    Variable wf: world -> Any.t * Any.t -> Prop.
     Variable le: world -> world -> Prop.
 
     Hypothesis le_PreOrder: PreOrder le.
@@ -1000,7 +983,7 @@ Section ADEQUACY.
         (exists (f_src f_tgt: _ -> itree _ _),
             (<<SRC: ms_src.(ModSem.fnsems) fn = Some (f_src)>>) /\
             (<<TGT: ms_tgt.(ModSem.fnsems) fn = Some (f_tgt)>>) /\
-            (<<SIM: sim_fsem le wf f_src f_tgt>>)).
+            (<<SIM: sim_fsem wf le f_src f_tgt>>)).
 
 
     Variant g_lift_rel
@@ -1009,18 +992,17 @@ Section ADEQUACY.
         w1
         (LE: le w0 w1)
         (MN: wf w1 (st_src0, st_tgt0))
-        (* (NMN: forall mn' (NIN: mn <> mn'), st_src mn' = st_tgt mn') *)
+        (* (NMN: forall mn' (NIN: mn <> mn'), st_local mn' = st_local mn') *)
     .
 
     Variant my_r0:
       forall R0 R1 (RR: R0 -> R1 -> Prop), bool -> bool -> (itree eventE R0) -> (itree eventE R1) -> Prop :=
     | my_r0_intro
         w0
-        (st_src: Type := ms_src.(ModSem.state)) (st_tgt: Type := ms_tgt.(ModSem.state))
-        (itr_src: itree (Es st_src) Any.t)(itr_tgt: itree (Es st_tgt) Any.t)
+        (itr_src itr_tgt: itree Es Any.t)
         st_src0 st_tgt0 o_src o_tgt
-        (SIM: sim_itree le o_src o_tgt w0 wf (st_src0, itr_src) (st_tgt0, itr_tgt))
-        (* (STATE: forall mn' (MN: mn <> mn'), st_src mn' = st_tgt mn') *)
+        (SIM: sim_itree wf le o_src o_tgt w0 (st_src0, itr_src) (st_tgt0, itr_tgt))
+        (* (STATE: forall mn' (MN: mn <> mn'), st_local mn' = st_local mn') *)
       :
         my_r0 (fun '(st_src, ret_src) '(st_tgt, ret_tgt) =>
                   g_lift_rel w0 st_src st_tgt /\ ret_src = ret_tgt)
@@ -1046,16 +1028,16 @@ Section ADEQUACY.
         | |- ?P o_src o_tgt w p p0 => set P
         end.
         revert o_src o_tgt w p p0 SIM.
-        eapply (@sim_itree_ind world le _ _ Any.t Any.t wf (lift_rel le w0 wf (@eq Any.t)) P); subst P; ss; i; clarify.
+        eapply (@sim_itree_ind world wf le Any.t Any.t (lift_rel wf le w0 (@eq Any.t)) P); subst P; ss; i; clarify.
 
         - rr in RET. des. step. splits; auto. econs; et.
         - hexploit (fnsems_find_iff fn). i. des.
-          { step. rewrite interp_Es_bind.  steps. rewrite NONE. unfold unwrapU, triggerUB. (* step.: coq bug?????? *) rewrite interp_Es_bind. step.  ss. }
+          { step. rewrite interp_Es_bind.  steps. rewrite NONE. unfold unwrapU, triggerUB. grind. step. ss. }
           { hexploit (SIM (varg) (varg)); et. i. des. ired_both. 
-            steps. rewrite interp_Es_bind. rewrite SRC. rewrite TGT. unfold unwrapU. ired_both.
+            steps. grind. rewrite SRC. rewrite TGT. unfold unwrapU. ired_both.
             apply simg_progress_flag.
             guclo bindC_spec. econs.
-            { gbase. eapply CIH. econs; ss. rewrite bind_ret_l. rewrite bind_ret_r. et. }
+            { gbase. eapply CIH. econs; ss. grind. et. }
             { i. ss. destruct vret_src, vret_tgt. des; clarify. inv SIM0.
               hexploit K; et. i. des. pclearbot. ired_both.
               steps. gbase. eapply CIH. econs; et.
@@ -1095,10 +1077,7 @@ Section ADEQUACY.
       unfold ModSem.initial_itr, assume. generalize "main" as fn. i.
       hexploit (fnsems_find_iff fn). i. des.
       { steps. unshelve esplits; et. unfold ITree.map, unwrapU, triggerUB. steps.
-        rewrite NONE. steps. ss. grind.
-        rewrite ! interp_Es_bind. grind.
-        rewrite interp_Es_eventE. grind.
-        gstep. econs; et. i. destruct x0. }
+        rewrite NONE. steps. ss. }
       { 
         inv H. 
         hexploit (SIM (initial_arg) (initial_arg)) ; et; cycle 1. i. des.
@@ -1110,7 +1089,19 @@ Section ADEQUACY.
         { i. destruct vret_src, vret_tgt. des; clarify. steps. }
       }
     Qed.
+
+    Definition wf_lift wf :=
+      fun (w:world) => 
+      (fun '(src, tgt) =>
+        match (Any.split src), (Any.split tgt) with
+        | Some (l1, r1), Some (l2, r2) => l1 = l2 /\ wf w (r1, r2)
+        | _, _ => wf w (src, tgt)
+        end
+      ).
+
   End SEMPAIR.
+
+
 
 
   (*  *)
@@ -1122,13 +1113,14 @@ Section ADEQUACY.
   Proof. 
   (* Admitted. *)
     ii. revert PR.
-    generalize (ModAdd.add_list ctx) as CTX.
+    generalize (ModAdd.add_list ctx) as CTX. 
+    (* context doesn't need to be a list anymore. Change the definition later. *)
     clear ctx. ii.
     unfold ModAdd.compile, Mod.enclose in *.
     destruct (classic (Mod.wf (ModAdd.add (CTX) md_src))).
     2:{ eapply ModSem.compile_not_wf. ss. }
-    pose (sk_tgt := (Mod.sk (Mod.add (CTX) md_tgt))).
-    pose (sk_src := (Mod.sk (Mod.add (CTX) md_src))).
+    pose (sk_tgt := (Mod.sk (ModAdd.add (CTX) md_tgt))).
+    pose (sk_src := (Mod.sk (ModAdd.add (CTX) md_src))).
     assert (SKEQ: sk_tgt = sk_src).
     { unfold sk_src, sk_tgt. ss. f_equal.
       inv SIM. auto. }
@@ -1146,7 +1138,7 @@ Section ADEQUACY.
       unfold Sk.wf in *. ss. eapply Permutation.Permutation_NoDup; [|et].
       eapply Permutation.Permutation_map. eapply Sk.SkSort.sort_permutation. }
     i. inv H0. des.
-    assert (WFTGT: Mod.wf (Mod.add (CTX) md_tgt)).
+    assert (WFTGT: Mod.wf (ModAdd.add (CTX) md_tgt)).
     { rr. ss. 
       match goal with
         | H: NoDup ?l0 |- NoDup ?l1 => replace l1 with l0
@@ -1154,37 +1146,59 @@ Section ADEQUACY.
       rewrite sim_sk. et.
     }
     (* simpl in PR. rewrite <- sim_sk in PR.    *)
-    revert PR.
+    (* revert PR.
 
-    (* generalize (Mod.get_modsem (ModAdd.add (CTX) md_src) (Sk.canon (Mod.sk (ModAdd.add (CTX) md_src)))) as ms_src.
-    generalize (Mod.get_modsem (ModAdd.add (CTX) md_tgt) (Sk.canon (Mod.sk (ModAdd.add (CTX) md_tgt)))) as ms_tgt. *)
-    i.
+    generalize (Mod.get_modsem (ModAdd.add (CTX) md_src) (Sk.canon (Mod.sk (ModAdd.add (CTX) md_src)))) as ms_src.
+    generalize (Mod.get_modsem (ModAdd.add (CTX) md_tgt) (Sk.canon (Mod.sk (ModAdd.add (CTX) md_tgt)))) as ms_tgt.
+    i. *)
 
     eapply adequacy_local_aux in PR; et.
     
-    { admit. }
-      (* ss. ii. 
+    { 
       (* previous version is proved by second branch (exists mn, ... ) which doesn't exists anymore *)
-    
-      fold sk_src sk_tgt.
+      ss. ii. fold sk_src sk_tgt. rewrite <- SKEQ.  
       (* revert_until SKEQ. *)
       (* pattern (Sk.sort sk_tgt) at 1. *)
       (* rewrite <- SKEQ. rewrite ! alist_find_app_o. des_ifs. *)
 
-      esplits. 
-      generalize (ModSem.add_fnsems (Mod.get_modsem (CTX) (Sk.sort sk_src))
-      (Mod.get_modsem md_src (Sk.sort sk_src)) fn) as o_src. 
-      generalize (ModSem.add_fnsems (Mod.get_modsem (CTX) (Sk.sort sk_tgt))
-      (Mod.get_modsem md_tgt (Sk.sort sk_tgt)) fn) as o_tgt.
+      esplits. instantiate (1:= le). Check (wf_lift wf).
+      instantiate (1:= wf_lift wf).
+      unfold sim_fnsem in *.
+      (* revert fn. *)
+
+      hexploit (sim_fnsems fn). i.
       
-      i. destruct (ModSem.fnsems ms_src fn); cycle 1.
+      revert_until SKEQ.
+      generalize (Mod.get_modsem md_src (Sk.sort sk_tgt)) as ms_src. 
+      generalize (Mod.get_modsem md_tgt (Sk.sort sk_tgt)) as ms_tgt.
+      unfold ModSemAdd.add_fnsems.
+      i. des_ifs; et; right.
+      - exists (fun _ : Any.t => triggerUB), (fun _ : Any.t => triggerUB). 
+        esplits; et. 
+        unfold sim_fsem, "==>". i.
+        ginit. gstep. econs. ss.
+      - exists (fun args : Any.t => translate ModSemAdd.emb_l (i args)), (fun args : Any.t => translate ModSemAdd.emb_l (i args)).
+        esplits; et.
+        unfold sim_fsem, "==>". i. rewrite H1.
+        unfold wf_lift in SIMMRS. des_ifs.
+        +  
+        ginit. gstep. econs.
+
+      generalize (ModSemAdd.add_fnsems (Mod.get_modsem (CTX) (Sk.sort sk_tgt)) ms_src) as o_src. 
+      generalize (ModSemAdd.add_fnsems (Mod.get_modsem (CTX) (Sk.sort sk_tgt)) ms_tgt) as o_tgt.
+      i.
+      destruct o_src, o_tgt; et; right.
+      - exists i, i0. esplits; et. apply sim_fnsems. 
+      destruct (ModSem.fnsems ms_src fn); cycle 1.
       - left. et.
       - right. exists i.
     
       
       
       exists i. destruct o_tgt; cycle 1. 
-        + eexists. splits; et.  
+        + eexists. splits; et. instantiate (1:= le). instantiate (1:=wf).
+          splits.
+          *     
         + exists i0. splits; et.
           unfold sim_fsem, respectful'. ii.
 
@@ -1221,7 +1235,7 @@ Section ADEQUACY.
         }
         { ss. inv H. ss. clarify. }
       }
-    } *)
+    }
     { exists w_init. econs.
       { refl. }
       { ss. 
