lib/Optics.v
@@ -27,60 +27,11 @@ End Store.
 
 Module Lens.
 
-  (* Lens is just a coalgebra of the Store comonad *)
-
-  (* Record isLens {S V} (l : S -> Store.t V S) : Prop :=
-    { counit : Store.counit ∘ l = id
-    ; coaction : Store.map l ∘ l = Store.cojoin ∘ l
-    }. *)
-
   Definition t S V := S -> Store.t V S.
-  (* Definition t S V := {l : S -> Store.t V S | isLens l}. *)
 
   Definition view {S V} : t S V -> S -> V := fun l s => fst (l s).
   Definition set {S V} : t S V -> V -> S -> S := fun l a s => snd (l s) a.
   Definition modify {S V} : t S V -> (V -> V) -> (S -> S) := fun l f s => Lens.set l (f (Lens.view l s)) s.
-
-  (* Lemma view_set {S V} (l : t S V) : forall v s, view l (set l v s) = v.
-  Proof.
-    destruct l as [l [H1 H2]]. 
-    unfold view, set; ss.
-    i. hspecialize H2 with s. cong snd in H2. hspecialize H2 with v. ss.
-    unfold compose in H2. rewrite H2. ss.
-  Qed.
-
-  Lemma set_view {S V} (l : t S V) : forall s, set l (view l s) s = s.
-  Proof.
-    destruct l as [l [H1 H2]]. unfold view, set; ss.
-    i. hspecialize H1 with s. ss.
-  Qed.
-
-  Lemma set_set {S V} (l : t S V) : forall v v' s, set l v' (set l v s) = set l v' s.
-  Proof.
-    destruct l as [l [H1 H2]]. unfold view, set; ss.
-    i. hspecialize H2 with s. cong snd in H2. hspecialize H2 with v. ss.
-    unfold compose in H2. rewrite H2. ss.
-  Qed.
-
-  Definition compose {A B C} : t A B -> t B C -> t A C.
-  Proof.
-    intros l1 l2.
-    exists (fun a => (view l2 (view l1 a), fun c => set l1 (set l2 c (view l1 a)) a)).
-    constructor.
-    - extensionalities s. cbn. rewrite ! set_view. ss.
-    - extensionalities s. unfold Store.map, Store.cojoin, compose; ss. f_equal.
-      extensionalities c. f_equal.
-      + rewrite ! view_set. ss.
-      + extensionalities c'. rewrite view_set, ! set_set. ss.
-  Defined.
-
-  Lemma compose_assoc A B C D (l1 : t A B) (l2 : t B C) (l3 : t C D) :
-    (compose (compose l1 l2) l3) = compose l1 (compose l2 l3).
-  Proof.
-    eapply eq_sig_hprop.
-    - i. eapply proof_irrelevance.
-    - ss.
-  Qed. *)
 
 End Lens.
 
@@ -88,30 +39,18 @@ Section PRODUCT_LENS.
 
   (* Context {A B : Type}. *)
 
-  Definition anypair (oa ob: option Any.t) : option Any.t :=
-    match oa, ob with
-    | Some a, Some b => Some (Any.pair a b)
-    | _, _ => None
-    end.
+  Definition fstl : Lens.t Any.t Any.t :=
+    (fun ab => 
+      match Any.split ab with
+      | Some (a, b) => (a, (fun a' => Any.pair a' b)) 
+      | None => (tt↑, (fun _ => tt↑))
+      end).
 
-  Definition fstl : Lens.t (option Any.t) (option Any.t) :=
-    (fun oab => 
-    match oab with
-    | Some ab => match Any.split ab with
-                | Some (a, b) => (Some a, (fun oa => anypair oa (Some b))) 
-                | None => (None, (fun _ => None))
-                end       
-    | None => (None, (fun _ => None))
-    end).
-
-  Definition sndl : Lens.t (option Any.t) (option Any.t) :=
-    (fun oab => 
-    match oab with
-    | Some ab => match Any.split ab with
-                | Some (a, b) => (Some b, (fun ob => anypair (Some a) ob)) 
-                | None => (None, (fun _ => None))
-                end       
-    | None => (None, (fun _ => None))
-    end).
+  Definition sndl : Lens.t Any.t Any.t :=
+    (fun ab => 
+      match Any.split ab with
+      | Some (a, b) => (b, (fun b' => Any.pair a b')) 
+      | None => (tt↑, (fun _ => tt↑))
+      end).
 
 End PRODUCT_LENS.
